ReTierProofAggregation.v
@@ -2,17 +2,19 @@ Require Import ReTierSyntax.
 Require Import ReTierStaticSemantics.
 Require Import ReTierDynamicSemantics.
 
-Lemma aggregation_multiple : forall context p0 p1 peers v v_agg v_type,
-  getTieMult context (p0, p1) = Some multiple ->
+Lemma aggregation_multiple:
+  forall typing ties Psi Delta Gamma P p0 p1 peers v v_agg v_type,
+  ties (p0, p1) = Some multiple ->
   value v ->
   transmittable_type v_type ->
-  context |- v \in v_type ->
-  Phi (getTies context) p0 p1 peers v v_type = Some v_agg ->
-  value v_agg /\ transmittable_type (List v_type) /\ context |- v_agg \in (List v_type).
+  typing; ties; Psi; Delta; Gamma; P |- v : v_type ->
+  Phi ties p0 p1 peers v v_type = Some v_agg ->
+    value v_agg /\
+    transmittable_type (List v_type) /\
+    typing; ties; Psi; Delta; Gamma; P |- v_agg : List v_type.
 Proof.
 intros until v_type.
 intros H_multiple H_value H_transmittable H_type H_Phi.
-unfold getTieMult in H_multiple.
 generalize dependent v_agg.
 induction peers as [| peer0 peers IH_peers ]; intros v_agg H_Phi.
 - simpl in H_Phi.
@@ -22,7 +24,7 @@ induction peers as [| peer0 peers IH_peers ]; intros v_agg H_Phi.
   + apply v_nil.
   + apply U_List. assumption.
   + apply T_Nil.
-- assert (H : exists v_agg, Phi (getTies context) p0 p1 peers v v_type = Some v_agg).
+- assert (H : exists v_agg, Phi ties p0 p1 peers v v_type = Some v_agg).
   + clear IH_peers H_Phi.
     induction peers as [| peer1 peers IH_peers ].
     * simpl.
@@ -36,7 +38,7 @@ induction peers as [| peer0 peers IH_peers ]; intros v_agg H_Phi.
       exists (cons v v_agg2).
       reflexivity.
   + inversion H as [ v_agg2 H_Phi2 ].
-    simpl in IH_peers, H_Phi, H_Phi2.
+    simpl in H_Phi.
     rewrite H_multiple in H_Phi.
     rewrite H_Phi2 in H_Phi.
     rewrite H_Phi2 in IH_peers.
@@ -52,17 +54,19 @@ induction peers as [| peer0 peers IH_peers ]; intros v_agg H_Phi.
       reflexivity.
 Qed.
 
-Lemma aggregation_optional : forall context p0 p1 peers v v_agg v_type,
-  getTieMult context (p0, p1) = Some optional ->
+Lemma aggregation_optional:
+  forall typing ties Psi Delta Gamma P p0 p1 peers v v_agg v_type,
+  ties (p0, p1) = Some optional ->
   value v ->
   transmittable_type v_type ->
-  context |- v \in v_type ->
-  Phi (getTies context) p0 p1 peers v v_type = Some v_agg ->
-  value v_agg /\ transmittable_type (Option v_type) /\ context |- v_agg \in (Option v_type).
+  typing; ties; Psi; Delta; Gamma; P |- v : v_type ->
+  Phi ties p0 p1 peers v v_type = Some v_agg ->
+    value v_agg /\
+    transmittable_type (Option v_type) /\
+    typing; ties; Psi; Delta; Gamma; P |- v_agg : Option v_type.
 Proof.
 intros until v_type.
 intros H_multiple H_value H_transmittable H_type H_Phi.
-unfold getTieMult in H_multiple.
 destruct peers.
 - simpl in H_Phi.
   rewrite H_multiple in H_Phi.
@@ -83,17 +87,19 @@ destruct peers.
     congruence.
 Qed.
 
-Lemma aggregation_single : forall context p0 p1 peers v v_agg v_type,
-  getTieMult context (p0, p1) = Some single ->
+Lemma aggregation_single:
+  forall typing ties Psi Delta Gamma P p0 p1 peers v v_agg v_type,
+  ties (p0, p1) = Some single ->
   value v ->
   transmittable_type v_type ->
-  context |- v \in v_type ->
-  Phi (getTies context) p0 p1 peers v v_type = Some v_agg ->
-  value v_agg /\ transmittable_type v_type /\ context |- v_agg \in v_type.
+  typing; ties; Psi; Delta; Gamma; P |- v : v_type ->
+  Phi ties p0 p1 peers v v_type = Some v_agg ->
+    value v_agg /\
+    transmittable_type v_type /\
+    typing; ties; Psi; Delta; Gamma; P |- v_agg : v_type.
 Proof.
 intros until v_type.
 intros H_multiple H_value H_transmittable H_type H_Phi.
-unfold getTieMult in H_multiple.
 destruct peers.
 - simpl in H_Phi.
   rewrite H_multiple in H_Phi.
@@ -109,19 +115,22 @@ destruct peers.
     congruence.
 Qed.
 
-Lemma aggregation : forall context p0 p1 peers v v_agg v_type v_agg_type,
-  getTieMult context (p0, p1) <> None ->
-  getTieMult context (p0, p1) <> Some mNone ->
-  Phi (getTies context) p0 p1 peers v v_type = Some v_agg ->
-  phi context p0 p1 v_type = Some v_agg_type ->
+Lemma aggregation:
+  forall typing ties Psi Delta Gamma P p0 p1 peers v v_agg v_type v_agg_type,
+  ties (p0, p1) <> None ->
+  ties (p0, p1) <> Some mNone ->
+  Phi ties p0 p1 peers v v_type = Some v_agg ->
+  phi ties p0 p1 v_type = Some v_agg_type ->
   value v ->
   transmittable_type v_type ->
-  context |- v \in v_type ->
-  value v_agg /\ transmittable_type v_agg_type /\ context |- v_agg \in v_agg_type.
+  typing; ties; Psi; Delta; Gamma; P |- v : v_type ->
+    value v_agg /\
+    transmittable_type v_agg_type /\
+    typing; ties; Psi; Delta; Gamma; P |- v_agg : v_agg_type.
 Proof.
 intros until v_agg_type.
 intros H_tie0 H_tie1 H_Phi H_phi_type H_value H_transmittable H_type.
-case_eq (getTieMult context (p0, p1)).
+case_eq (ties (p0, p1)).
 - intros multiplicity H_tie.
   unfold phi in H_phi_type.
   rewrite H_tie in H_phi_type.
