ReTierProofContext.v
@@ -5,8 +5,8 @@ Require Import ReTierStaticSemantics.
 Lemma transmittable_value_typing : forall typing ties Psi Delta Delta' Gamma Gamma' P P' v T,
   value v ->
   transmittable_type T ->
-  Context typing ties Psi Delta Gamma P |- v \in T ->
-  Context typing ties Psi Delta' Gamma' P' |- v \in T.
+  typing; ties; Psi; Delta; Gamma; P |- v : T ->
+  typing; ties; Psi; Delta'; Gamma'; P' |- v : T.
 Proof.
 intros until T.
 intros H_value H_transmittable H_typing.
@@ -104,7 +104,7 @@ Qed.
 
 
 Lemma free_in_context_t : forall typing ties Psi Delta Gamma P t T x,
-  Context typing ties Psi Delta Gamma P |- t \in T ->
+  typing; ties; Psi; Delta; Gamma; P |- t : T ->
   (appears_free_in_t_locality x t LocalOrRemoteVar ->
    exists T' P', Gamma x = Some T' \/ Delta x = Some (T' on P')) /\
   (appears_free_in_t_locality x t RemoteVar ->
@@ -146,9 +146,8 @@ induction t; intros; inversion H_typing; subst; split; intros H_free_x; simpl in
 - case_eq (beq_id x i); intros H_eq.
   + rewrite beq_id_eq in H_eq.
     subst.
-    unfold getVarEnv, getVarEnv, getPlaceEnv, getPeer in H1.
     exists T, P.
-    destruct H1.
+    destruct H6.
     * left. assumption.
     * destruct H.
       right; assumption.
@@ -169,8 +168,7 @@ induction t; intros; inversion H_typing; subst; split; intros H_free_x; simpl in
 - destruct H_free_x.
   + eapply IHt1; eassumption.
   + eapply IHt2; eassumption.
-- simpl in H_free_x.
-  eapply IHt with (Gamma := emptyVarEnv) in H_free_x; try eassumption.
+- eapply IHt with (Gamma := emptyVarEnv) in H_free_x; try eassumption.
   destruct
       H_free_x as [ T' H_lookup ],
       H_lookup as [ P' H_lookup ],
@@ -179,8 +177,7 @@ induction t; intros; inversion H_typing; subst; split; intros H_free_x; simpl in
     congruence.
   + exists T', P'.
     right. assumption.
-- simpl in H_free_x.
-  eapply IHt with (Gamma := emptyVarEnv) in H_free_x; try eassumption.
+- eapply IHt with (Gamma := emptyVarEnv) in H_free_x; try eassumption.
   destruct
       H_free_x as [ T' H_lookup ],
       H_lookup as [ P' H_lookup ],
@@ -326,7 +323,7 @@ Qed.
 
 Lemma free_in_context_s : forall typing ties Psi Delta s x,
    appears_free_in_s x s ->
-   PlacementContext typing ties Psi Delta |~ s ->
+   typing; ties; Psi; Delta |- s ->
    exists S, Delta x = Some S.
 Proof.
 intros until x.
@@ -334,7 +331,7 @@ intros H_free_x H_typing.
 generalize dependent Delta.
 induction s; intros; inversion H_typing; subst; simpl in H_free_x.
 - case_eq (beq_id x i); intros H_eq; rewrite H_eq in H_free_x.
-  + eapply free_in_context_t in H5 as H_lookup; try eassumption.
+  + eapply free_in_context_t in H8 as H_lookup; try eassumption.
     destruct H_lookup as [ H_lookup_Gamma H_lookup_Delta ].
     destruct H_lookup_Gamma as [ T' H_lookup ]. try eassumption.
     destruct
@@ -345,7 +342,7 @@ induction s; intros; inversion H_typing; subst; simpl in H_free_x.
     * exists (T' on P').
       assumption.
   + destruct H_free_x as [ H_free_x | H_free_x ].
-    * { eapply free_in_context_t in H5 as H_lookup; try eassumption.
+    * { eapply free_in_context_t in H8 as H_lookup; try eassumption.
         destruct H_lookup as [ H_lookup_Gamma H_lookup_Delta ].
         destruct H_lookup_Gamma as [ T' H_lookup ]. try eassumption.
         destruct
@@ -370,12 +367,12 @@ Qed.
 
 
 Lemma context_invariance_t : forall typing ties Psi Delta Delta' Gamma Gamma' P t T,
-  Context typing ties Psi Delta Gamma P |- t \in T ->
+  typing; ties; Psi; Delta; Gamma; P |- t : T ->
   (forall x, appears_free_in_t_locality x t LocalOrRemoteVar ->
    Gamma x = Gamma' x /\ (Gamma x = None -> Delta x = Delta' x)) ->
   (forall x, appears_free_in_t_locality x t RemoteVar ->
    Delta x = Delta' x) ->
-  Context typing ties Psi Delta' Gamma' P |- t \in T.
+  typing; ties; Psi; Delta'; Gamma'; P |- t : T.
 Proof.
 intros until T.
 intros H_typing H_free_x_Gamma H_free_x_Delta.
@@ -383,9 +380,9 @@ generalize dependent Gamma.
 generalize dependent Gamma'.
 generalize dependent T.
 generalize dependent P.
-induction t; intros; inversion H_typing.
-- eapply IHt in H4.
-  + apply T_Abs. simpl. eassumption.
+induction t; intros; inversion H_typing; subst.
+- eapply IHt in H9.
+  + apply T_Abs. eassumption.
   + intros y H_free_y.
     apply H_free_x_Delta.
     simpl.
@@ -398,22 +395,20 @@ induction t; intros; inversion H_typing.
       simpl.
       rewrite H_eq.
       assumption.
-- eapply IHt1 in H2.
-  + eapply IHt2 in H4.
+- eapply IHt1 in H7.
+  + eapply IHt2 in H9.
     * eapply T_App; eassumption.
     * intros. apply H_free_x_Delta. simpl. right. assumption.
     * intros. apply H_free_x_Gamma. simpl. right. assumption.
   + intros. apply H_free_x_Delta. simpl. left. assumption.
   + intros. apply H_free_x_Gamma. simpl. left. assumption.
-- simpl in H1.
-  apply T_Var.
-  simpl.
+- apply T_Var.
   specialize H_free_x_Gamma with i.
   simpl in H_free_x_Gamma.
   rewrite beq_id_refl in H_free_x_Gamma.
   destruct H_free_x_Gamma as [ H_Gamma H_Gamma_Delta ]; try reflexivity.
   rewrite <- H_Gamma.
-  destruct H1 as [ H_lookup_Gamma | H_lookup_Delta ].
+  destruct H6 as [ H_lookup_Gamma | H_lookup_Delta ].
   + left. assumption.
   + destruct H_lookup_Delta as [ H_lookup_Gamma H_lookup_Delta ].
     apply H_Gamma_Delta in H_lookup_Gamma as H_Delta.
@@ -421,31 +416,31 @@ induction t; intros; inversion H_typing.
     right. split; assumption.
 - apply T_Unit.
 - apply T_None.
-- eapply IHt in H1.
+- eapply IHt in H6.
   + eapply T_Some; eassumption.
   + intros. apply H_free_x_Delta. assumption.
   + intros. apply H_free_x_Gamma. assumption.
 - apply T_Nil.
-- eapply IHt1 in H2.
-  + eapply IHt2 in H4.
+- eapply IHt1 in H7.
+  + eapply IHt2 in H9.
     * eapply T_Cons; eassumption.
     * intros. apply H_free_x_Delta. simpl. right. assumption.
     * intros. apply H_free_x_Gamma. simpl. right. assumption.
   + intros. apply H_free_x_Delta. simpl. left. assumption.
   + intros. apply H_free_x_Gamma. simpl. left. assumption.
-- eapply IHt in H3.
+- eapply IHt in H2.
   + eapply T_AsLocal; eassumption.
   + intros.
     apply H_free_x_Delta.
     simpl.
-    apply appears_free_locally_or_remotely in H8.
+    apply appears_free_locally_or_remotely in H.
     assumption.
   + intros.
     split; try reflexivity.
     intros.
     apply H_free_x_Delta. simpl. assumption.
-- eapply IHt1 in H5.
-  + eapply IHt2 in H8.
+- eapply IHt1 in H9.
+  + eapply IHt2 in H12.
     * eapply T_AsLocalFrom; eassumption.
     * intros. apply H_free_x_Delta. simpl. right. assumption.
     * intros. apply H_free_x_Gamma. simpl. right. assumption.
@@ -453,14 +448,14 @@ induction t; intros; inversion H_typing.
     apply H_free_x_Delta.
     simpl.
     left.
-    apply appears_free_locally_or_remotely in H9.
+    apply appears_free_locally_or_remotely in H.
     assumption.
   + intros.
     split; try reflexivity.
     intros.
     apply H_free_x_Delta. simpl. left. assumption.
-- eapply IHt1 in H7.
-  + eapply IHt2 in H9.
+- eapply IHt1 in H11.
+  + eapply IHt2 in H13.
     * eapply T_Comp; eassumption.
     * { intros y H_free_y.
         apply H_free_x_Delta.
@@ -488,9 +483,9 @@ induction t; intros; inversion H_typing.
     apply H_free_x_Gamma.
     simpl.
     destruct (beq_id y i); left; assumption.
-- eapply IHt1 in H9.
-  + eapply IHt2 in H10.
-    * { eapply IHt3 in H12.
+- eapply IHt1 in H13.
+  + eapply IHt2 in H14.
+    * { eapply IHt3 in H16.
         - eapply T_ComFrom; eassumption.
         - intros y H_free_y.
           apply H_free_x_Delta.
@@ -527,11 +522,11 @@ induction t; intros; inversion H_typing.
     apply H_free_x_Gamma.
     simpl.
     destruct (beq_id y i); left; assumption.
-- eapply IHt in H1.
+- eapply IHt in H6.
   + eapply T_Signal; eassumption.
   + intros. apply H_free_x_Delta. assumption.
   + intros. apply H_free_x_Gamma. assumption.
-- eapply IHt in H1.
+- eapply IHt in H6.
   + eapply T_ReactiveVar; eassumption.
   + intros. apply H_free_x_Delta. assumption.
   + intros. apply H_free_x_Gamma. assumption.
@@ -539,8 +534,8 @@ induction t; intros; inversion H_typing.
   + eapply T_Now; eassumption.
   + intros. apply H_free_x_Delta. assumption.
   + intros. apply H_free_x_Gamma. assumption.
-- eapply IHt1 in H2.
-  + eapply IHt2 in H4.
+- eapply IHt1 in H7.
+  + eapply IHt2 in H9.
     * eapply T_Set; eassumption.
     * intros. apply H_free_x_Delta. simpl. right. assumption.
     * intros. apply H_free_x_Gamma. simpl. right. assumption.
@@ -553,18 +548,17 @@ Qed.
 
 
 Lemma context_invariance_s : forall typing ties Psi Delta' Delta s,
-  PlacementContext typing ties Psi Delta |~ s ->
+  typing; ties; Psi; Delta |- s ->
   (forall x, appears_free_in_s x s -> Delta x = Delta' x) ->
-  PlacementContext typing ties Psi Delta' |~ s.
+  typing; ties; Psi; Delta' |- s.
 Proof.
 intros until s.
 intros H_typing H_free_x.
 generalize dependent Delta.
 generalize dependent Delta'.
-induction s; (intros; inversion H_typing; subst).
-- eapply IHs in H2.
+induction s; intros; inversion H_typing; subst.
+- eapply IHs in H5.
   + eapply T_Place; try eassumption.
-    simpl.
     eapply context_invariance_t; try eassumption; intros.
     * split; try reflexivity.
       intros.
@@ -589,7 +583,7 @@ Qed.
 
 
 Lemma typable_empty_closed_t : forall typing ties Psi P t T,
-  Context typing ties Psi emptyPlaceEnv emptyVarEnv P |- t \in T ->
+  typing; ties; Psi; emptyPlaceEnv; emptyVarEnv; P |- t : T ->
   closed_t t.
 Proof.
 unfold closed_t, not.
@@ -603,7 +597,7 @@ Qed.
 
 
 Lemma typable_empty_closed_s : forall typing ties Psi s,
-  PlacementContext typing ties Psi emptyPlaceEnv |~ s ->
+  typing; ties; Psi; emptyPlaceEnv |- s ->
   closed_s s.
 Proof.
 unfold closed_t, not.
