Test_ReTierStaticSemantics.v
@@ -19,7 +19,6 @@ Require Import ReTierSyntax.
 Definition testPsi1: reactEnv   := reactUpdate (Reactive 0) Unit reactEmpty.
 Definition testGamma1: varEnv   := idUpdate (Id "x") Tnat (idUpdate (Id "y") Unit idEmpty).
 Definition testDelta1: placeEnv := idUpdate (Id "x") (Unit on (Peer "px")) idEmpty.
-Definition testPlCont1_NoTies := PlacementContext noPeers noTies testPsi1 testDelta1.
 Definition testTies1  :=  (tie_update (Peer "p0" *-> Peer "pm")
                             (tie_update (Peer "p0" ?-> Peer "po")
                               (tie_update (Peer "p0" S-> Peer "ps")
@@ -31,27 +30,25 @@ Definition testPeerTyping1 := (pT_update (PeerInst 4) (Peer "pm")
                                     (pT_update (PeerInst 1) (Peer "pn")
                                       (pT_update (PeerInst 0) (Peer "p0")
                                       noPeers))))).
-Definition testTies1Context := tiesToContext testTies1 (Peer "p0").
-Definition testPeerTyping1Ties1Context := 
-              Context testPeerTyping1 testTies1 emptyReactEnv emptyPlaceEnv emptyVarEnv (Peer "p0").
-Definition testReactContext1 := reToContext testPsi1 (Peer "_").
 
 
-Example test_pltIsWellTyped_TEnd_1: emptyPlContext |~ pUnit.
+Example test_pltIsWellTyped_TEnd_1:
+  noPeers; noTies; emptyReactEnv; emptyPlaceEnv |- pUnit.
 Proof. apply T_End. Qed.
 
 
-Example test_pltIsWellTyped_TEnd_2: testPlCont1_NoTies |~ pUnit.
+Example test_pltIsWellTyped_TEnd_2:
+  noPeers; noTies; testPsi1; testDelta1 |- pUnit.
 Proof. apply T_End. Qed.
 
 
-(* Tested earlier because next test's proof relies inference rule T_Unit it. *)
-Example test_hasType_TUnit_1: (emptyContext |- unit \in Unit).
+Example test_hasType_TUnit_1:
+  noPeers; noTies; emptyReactEnv; emptyPlaceEnv; emptyVarEnv; Peer "dummy" |- unit : Unit.
 Proof. apply T_Unit. Qed.
 
 
 Example test_pltIsWellTyped_TPlace_1:
-  testPlCont1_NoTies |~ (placed (Id "x") (Unit on (Peer "px")) unit pUnit).
+  noPeers; noTies; testPsi1; testDelta1 |- placed (Id "x") (Unit on (Peer "px")) unit pUnit.
 Proof.
   apply T_Place.
   - apply T_End.
@@ -59,39 +56,34 @@ Proof.
 Qed.
 
 
-Example test_hasType_TVar_normalVar_1: 
-    (veToContext testGamma1 (Peer "p1")) |- (idApp (Id "x")) \in Tnat.
+Example test_hasType_TVar_normalVar_1:
+  noPeers; noTies; emptyReactEnv; emptyPlaceEnv; testGamma1; Peer "p1" |- idApp (Id "x") : Tnat.
 Proof. apply T_Var. left. reflexivity. Qed.
 
 
 Example test_hasType_TVar_placedVar_2:
-    (peToContext testDelta1 (Peer "px")) |- (idApp (Id "x")) \in Unit.
+  noPeers; noTies; emptyReactEnv; testDelta1; emptyVarEnv; Peer "px" |- idApp (Id "x") : Unit.
 Proof. apply T_Var. right. split. - reflexivity. - reflexivity. Qed.
 
 
 Example test_hasType_TAbs_1: 
-    emptyContext |- (lambda (Id "x") Tnat unit) \in (Arrow Tnat Unit).
+    noPeers; noTies; emptyReactEnv; emptyPlaceEnv; emptyVarEnv; Peer "dummy" |- lambda (Id "x") Tnat unit : Tnat ~> Unit.
 Proof. apply T_Abs. apply T_Unit. Qed.
 
 
 Example test_hasType_TAbs_2: 
-    emptyContext |- (lambda (Id "x") Tnat (idApp (Id "x"))) \in (Arrow Tnat Tnat).
+    noPeers; noTies; emptyReactEnv; emptyPlaceEnv; emptyVarEnv; Peer "dummy" |- lambda (Id "x") Tnat (idApp (Id "x")) : Tnat ~> Tnat.
 Proof. apply T_Abs. apply T_Var. left. reflexivity. Qed.
 
 
 (** Tests variable shadowing **)
-Example test_hasType_TAbs_3:  
-    (testGamma1 (Id "x")) = Some Tnat /\ (veToContext testGamma1 (Peer "_"))
-    |- (lambda (Id "x") Unit (idApp (Id "x"))) \in (Arrow Unit Unit).
-Proof.
-  split.
-  - reflexivity.
-  - apply T_Abs. apply T_Var. left. reflexivity.
-Qed.
+Example test_hasType_TAbs_3:
+  noPeers; noTies; emptyReactEnv; emptyPlaceEnv; testGamma1; Peer "_" |- lambda (Id "x") Unit (idApp (Id "x")) : Unit ~> Unit.
+Proof. apply T_Abs. apply T_Var. left. reflexivity. Qed.
 
 
 Example test_hasType_TApp_1:
-    emptyContext |- (app (lambda (Id "x") Unit unit) unit) \in Unit.
+  noPeers; noTies; emptyReactEnv; emptyPlaceEnv; emptyVarEnv; Peer "dummy" |- app (lambda (Id "x") Unit unit) unit : Unit.
 Proof.
   apply T_App with (T2 := Unit).
   - apply T_Abs. apply T_Unit.
@@ -100,7 +92,7 @@ Qed.
 
 
 Example test_hasType_TApp_2: 
-    emptyContext |- (app (lambda (Id "x") Unit (idApp (Id "x"))) unit) \in Unit.
+  noPeers; noTies; emptyReactEnv; emptyPlaceEnv; emptyVarEnv; Peer "dummy" |- app (lambda (Id "x") Unit (idApp (Id "x"))) unit : Unit.
 Proof.
   apply T_App with (T2 := Unit).
   - apply T_Abs. apply T_Var. left. reflexivity.
@@ -109,12 +101,12 @@ Qed.
 
 
 Example test_hasType_TNil_1: 
-    emptyContext |- (nil Unit) \in List Unit.
+  noPeers; noTies; emptyReactEnv; emptyPlaceEnv; emptyVarEnv; Peer "dummy" |- nil Unit : List Unit.
 Proof. apply T_Nil. Qed.
 
 
 Example test_hasType_TCons_1: 
-    emptyContext |- (cons unit (nil Unit)) \in List Unit.
+  noPeers; noTies; emptyReactEnv; emptyPlaceEnv; emptyVarEnv; Peer "dummy" |- cons unit (nil Unit) : List Unit.
 Proof.
   apply T_Cons.
   - apply T_Unit.
@@ -123,322 +115,261 @@ Qed.
 
 
 Example test_hasType_TSome_1: 
-    emptyContext |- (some unit) \in Option Unit.
+    noPeers; noTies; emptyReactEnv; emptyPlaceEnv; emptyVarEnv; Peer "dummy" |- some unit : Option Unit.
 Proof. apply T_Some. apply T_Unit. Qed.
 
 
 Example test_hasType_TNone_1: 
-    emptyContext |- (none Unit) \in Option Unit.
+    noPeers; noTies; emptyReactEnv; emptyPlaceEnv; emptyVarEnv; Peer "dummy" |- none Unit : Option Unit.
 Proof. apply T_None. Qed.
 
 
 Example test_hasType_TPeer_1:
-    (* ensure test setup is correct ... *)
-    getPeerType testPeerTyping1Ties1Context (PeerInst 0) = Some (Peer "p0") /\
-    (* actual test ... *)
-    testPeerTyping1Ties1Context |- peerApp (PeerInst 0) \in Remote (Peer "p0").
-Proof.
-  split.
-  - reflexivity.
-  - apply T_Peer. reflexivity.
-Qed.
+  testPeerTyping1; testTies1; emptyReactEnv; emptyPlaceEnv; emptyVarEnv; Peer "p0" |- peerApp (PeerInst 0) : Remote (Peer "p0").
+Proof. apply T_Peer. reflexivity. Qed.
 
 
 Example test_hasType_TAsLocal_single_1:
-    (* ensure test setup is correct ... *)
-    getPeer testTies1Context = Peer "p0" /\
-    getTieMult testTies1Context (Peer "p0", Peer "ps") = Some single /\
-    (* actual test ... *)
-    testTies1Context |- (asLocal unit (Unit on (Peer "ps"))) \in Unit.
+  (* ensure test setup is correct ... *)
+  testTies1 (Peer "p0", Peer "ps") = Some single /\
+  (* actual test ... *)
+  noPeers; testTies1; emptyReactEnv; emptyPlaceEnv; emptyVarEnv; Peer "p0"
+    |- asLocal unit (Unit on (Peer "ps")) : Unit.
 Proof.
   split.
-  - reflexivity.  (* current peer set correctly *)
-  - split.
-    + reflexivity.  (* ties set up correctly *)
-    + { apply T_AsLocal with (P0 := (Peer "p0")).
-        - apply U_Unit.
-        - reflexivity.
-        - apply T_Unit.
-        - reflexivity.
-        - reflexivity.
-      }
+  - reflexivity. (* ties set up correctly *)
+  - apply T_AsLocal with (P0 := (Peer "p0")).
+    + apply U_Unit.
+    + apply T_Unit.
+    + reflexivity.
+    + reflexivity.
 Qed.
 
 
 Example test_hasType_TAsLocal_optional_1:
-    (* ensure test setup is correct ... *)
-    getPeer testTies1Context = Peer "p0" /\
-    getTieMult testTies1Context (Peer "p0", Peer "po") = Some optional /\
-    (* actual test ... *)
-    testTies1Context |- (asLocal unit (Unit on (Peer "po"))) \in Option Unit.
+  (* ensure test setup is correct ... *)
+  testTies1 (Peer "p0", Peer "po") = Some optional /\
+  (* actual test ... *)
+  noPeers; testTies1; emptyReactEnv; emptyPlaceEnv; emptyVarEnv; Peer "p0"
+    |- asLocal unit (Unit on (Peer "po")) : Option Unit.
 Proof.
   split.
-  - reflexivity.  (* current peer set correctly *)
-  - split.
-    + reflexivity.  (* ties set up correctly *)
-    + { apply T_AsLocal with (P0 := (Peer "p0")).
-        - apply U_Unit.
-        - reflexivity.
-        - apply T_Unit.
-        - reflexivity.
-        - reflexivity.
-      }
+  - reflexivity. (* ties set up correctly *)
+  - apply T_AsLocal with (P0 := (Peer "p0")).
+    + apply U_Unit.
+    + apply T_Unit.
+    + reflexivity.
+    + reflexivity.
 Qed.
 
 
 Example test_hasType_TAsLocal_multiple_1:
-    (* ensure test setup is correct ... *)
-    getPeer testTies1Context = Peer "p0" /\
-    getTieMult testTies1Context (Peer "p0", Peer "pm") = Some multiple /\
-    (* actual test ... *)
-    testTies1Context |- (asLocal unit (Unit on (Peer "pm"))) \in List Unit.
+  (* ensure test setup is correct ... *)
+  testTies1 (Peer "p0", Peer "pm") = Some multiple /\
+  (* actual test ... *)
+  noPeers; testTies1; emptyReactEnv; emptyPlaceEnv; emptyVarEnv; Peer "p0"
+    |- asLocal unit (Unit on (Peer "pm")) : List Unit.
 Proof.
   split.
   - reflexivity.  (* current peer set correctly *)
-  - split.
-    + reflexivity.  (* ties set up correctly *)
-    + { apply T_AsLocal with (P0 := (Peer "p0")).
-        - apply U_Unit.
-        - reflexivity.
-        - apply T_Unit.
-        - reflexivity.
-        - reflexivity.
-      }
+  - apply T_AsLocal with (P0 := (Peer "p0")).
+    + apply U_Unit.
+    + apply T_Unit.
+    + reflexivity.
+    + reflexivity.
 Qed.
 
 
 Example test_hasType_TAsLocalFrom_single_1:
-    (* ensure test setup is correct ... *)
-    getPeer testPeerTyping1Ties1Context = Peer "p0" /\
-    getPeerType testPeerTyping1Ties1Context (PeerInst 2) = Some (Peer "ps") /\
-    getTieMult testPeerTyping1Ties1Context (Peer "p0", Peer "ps") = Some single /\
-    (* actual test ... *)
-    testPeerTyping1Ties1Context |- asLocalFrom unit (Unit on (Peer "ps")) (peerApp (PeerInst 2)) \in Unit.
+  (* ensure test setup is correct ... *)
+  testPeerTyping1 (PeerInst 2) = Some (Peer "ps") /\
+  testTies1 (Peer "p0", Peer "ps") = Some single /\
+  (* actual test ... *)
+  testPeerTyping1; testTies1; emptyReactEnv; emptyPlaceEnv; emptyVarEnv; Peer "p0"
+    |- asLocalFrom unit (Unit on (Peer "ps")) (peerApp (PeerInst 2)) : Unit.
 Proof.
   split.
   - reflexivity.
   - split. 
     + reflexivity.
-    + { split.
-        - reflexivity.
-        - apply T_AsLocalFrom with (P0 := Peer "p0").
-          + apply U_Unit.
-          + reflexivity.
-          + apply T_Unit.
-          + reflexivity.
-          + apply T_Peer. reflexivity.
-      }
+    + apply T_AsLocalFrom with (P0 := Peer "p0").
+      * apply U_Unit.
+      * apply T_Unit.
+      * reflexivity.
+      * apply T_Peer. reflexivity.
 Qed.
 
 
 Example test_hasType_TAsLocalFrom_optional_1:
-    (* ensure test setup is correct ... *)
-    getPeer testPeerTyping1Ties1Context = Peer "p0" /\
-    getPeerType testPeerTyping1Ties1Context (PeerInst 3) = Some (Peer "po") /\
-    getTieMult testPeerTyping1Ties1Context (Peer "p0", Peer "po") = Some optional /\
-    (* actual test ... *)
-    testPeerTyping1Ties1Context |- asLocalFrom unit (Unit on (Peer "po")) (peerApp (PeerInst 3)) \in Unit.
+  (* ensure test setup is correct ... *)
+  testPeerTyping1 (PeerInst 3) = Some (Peer "po") /\
+  testTies1 (Peer "p0", Peer "po") = Some optional /\
+  (* actual test ... *)
+  testPeerTyping1; testTies1; emptyReactEnv; emptyPlaceEnv; emptyVarEnv; Peer "p0"
+    |- asLocalFrom unit (Unit on (Peer "po")) (peerApp (PeerInst 3)) : Unit.
 Proof.
   split.
   - reflexivity.
   - split. 
     + reflexivity.
-    + { split.
-        - reflexivity.
-        - apply T_AsLocalFrom with (P0 := Peer "p0").
-          + apply U_Unit.
-          + reflexivity.
-          + apply T_Unit.
-          + reflexivity.
-          + apply T_Peer. reflexivity.
-      }
+    + apply T_AsLocalFrom with (P0 := Peer "p0").
+      * apply U_Unit.
+      * apply T_Unit.
+      * reflexivity.
+      * apply T_Peer. reflexivity.
 Qed.
 
 
 Example test_hasType_TAsLocalFrom_multiple_1:
-    (* ensure test setup is correct ... *)
-    getPeer testPeerTyping1Ties1Context = Peer "p0" /\
-    getPeerType testPeerTyping1Ties1Context (PeerInst 4) = Some (Peer "pm") /\
-    getTieMult testPeerTyping1Ties1Context (Peer "p0", Peer "pm") = Some multiple /\
-    (* actual test ... *)
-    testPeerTyping1Ties1Context |- asLocalFrom unit (Unit on (Peer "pm")) (peerApp (PeerInst 4)) \in Unit.
+  (* ensure test setup is correct ... *)
+  testPeerTyping1 (PeerInst 4) = Some (Peer "pm") /\
+  testTies1 (Peer "p0", Peer "pm") = Some multiple /\
+  (* actual test ... *)
+  testPeerTyping1; testTies1; emptyReactEnv; emptyPlaceEnv; emptyVarEnv; Peer "p0"
+    |- asLocalFrom unit (Unit on (Peer "pm")) (peerApp (PeerInst 4)) : Unit.
 Proof.
   split.
   - reflexivity.
   - split. 
     + reflexivity.
-    + { split.
-        - reflexivity.
-        - apply T_AsLocalFrom with (P0 := Peer "p0").
-          + apply U_Unit.
-          + reflexivity.
-          + apply T_Unit.
-          + reflexivity.
-          + apply T_Peer. reflexivity.
-      }
+    + apply T_AsLocalFrom with (P0 := Peer "p0").
+      * apply U_Unit.
+      * apply T_Unit.
+      * reflexivity.
+      * apply T_Peer. reflexivity.
 Qed.
 
 
 Example test_hasType_TComp_single_1:
-    (* ensure test setup is correct ... *)
-    getPeer testTies1Context = Peer "p0" /\
-    getTieMult testTies1Context (Peer "p0", Peer "ps") = Some single /\
-    (* actual test ... *)
-    testTies1Context
-      |- asLocalIn (Id "x") unit unit (Unit on (Peer "ps")) \in Unit.
+  (* ensure test setup is correct ... *)
+  testTies1 (Peer "p0", Peer "ps") = Some single /\
+  (* actual test ... *)
+  noPeers; testTies1; emptyReactEnv; emptyPlaceEnv; emptyVarEnv; Peer "p0"
+    |- asLocalIn (Id "x") unit unit (Unit on (Peer "ps")) : Unit.
 Proof.
   split.
   - reflexivity.
-  - split.
+  - apply T_Comp with (P0 := Peer "p0") (T0 := Unit).
+    + apply U_Unit.
+    + apply U_Unit.
+    + apply T_Unit.
+    + apply T_Unit.
     + reflexivity.
-    + { apply T_Comp with (P0 := Peer "p0") (T0 := Unit).
-        - apply U_Unit.
-        - apply U_Unit.
-        - reflexivity.
-        - apply T_Unit.
-        - apply T_Unit.
-        - reflexivity.
-        - reflexivity.
-      }
+    + reflexivity.
 Qed.
 
 
 Example test_hasType_TComp_optional_1:
-    (* ensure test setup is correct ... *)
-    getPeer testTies1Context = Peer "p0" /\
-    getTieMult testTies1Context (Peer "p0", Peer "po") = Some optional /\
-    (* actual test ... *)
-    testTies1Context
-      |- asLocalIn (Id "x") unit unit (Unit on (Peer "po")) \in Option Unit.
+  (* ensure test setup is correct ... *)
+  testTies1 (Peer "p0", Peer "po") = Some optional /\
+  (* actual test ... *)
+  noPeers; testTies1; emptyReactEnv; emptyPlaceEnv; emptyVarEnv; Peer "p0"
+    |- asLocalIn (Id "x") unit unit (Unit on (Peer "po")) : Option Unit.
 Proof.
   split.
   - reflexivity.
-  - split.
+  - apply T_Comp with (P0 := Peer "p0") (T0 := Unit).
+    + apply U_Unit.
+    + apply U_Unit.
+    + apply T_Unit.
+    + apply T_Unit.
     + reflexivity.
-    + { apply T_Comp with (P0 := Peer "p0") (T0 := Unit).
-        - apply U_Unit.
-        - apply U_Unit.
-        - reflexivity.
-        - apply T_Unit.
-        - apply T_Unit.
-        - reflexivity.
-        - reflexivity.
-      }
+    + reflexivity.
 Qed.
 
 
 Example test_hasType_TComp_multiple_1:
-    (* ensure test setup is correct ... *)
-    getPeer testTies1Context = Peer "p0" /\
-    getTieMult testTies1Context (Peer "p0", Peer "pm") = Some multiple /\
-    (* actual test ... *)
-    testTies1Context
-      |- asLocalIn (Id "x") unit unit (Unit on (Peer "pm")) \in List Unit.
+  (* ensure test setup is correct ... *)
+  testTies1 (Peer "p0", Peer "pm") = Some multiple /\
+  (* actual test ... *)
+  noPeers; testTies1; emptyReactEnv; emptyPlaceEnv; emptyVarEnv; Peer "p0"
+    |- asLocalIn (Id "x") unit unit (Unit on (Peer "pm")) : List Unit.
 Proof.
   split.
   - reflexivity.
-  - split.
+  - apply T_Comp with (P0 := Peer "p0") (T0 := Unit).
+    + apply U_Unit.
+    + apply U_Unit.
+    + apply T_Unit.
+    + apply T_Unit.
     + reflexivity.
-    + { apply T_Comp with (P0 := Peer "p0") (T0 := Unit).
-        - apply U_Unit.
-        - apply U_Unit.
-        - reflexivity.
-        - apply T_Unit.
-        - apply T_Unit.
-        - reflexivity.
-        - reflexivity.
-      }
+    + reflexivity.
 Qed.
 
 
 Example test_hasType_TComp_single_2:
-    (* ensure test setup is correct ... *)
-    getPeer testTies1Context = Peer "p0" /\
-    getTieMult testTies1Context (Peer "p0", Peer "ps") = Some single /\
-    (* actual test ... *)
-    testTies1Context
-      |- asLocalIn (Id "x") unit (idApp (Id "x")) (Unit on (Peer "ps")) \in Unit.
+  (* ensure test setup is correct ... *)
+  testTies1 (Peer "p0", Peer "ps") = Some single /\
+  (* actual test ... *)
+  noPeers; testTies1; emptyReactEnv; emptyPlaceEnv; emptyVarEnv; Peer "p0"
+    |- asLocalIn (Id "x") unit (idApp (Id "x")) (Unit on (Peer "ps")) : Unit.
 Proof.
   split.
   - reflexivity.
-  - split.
+  - apply T_Comp with (P0 := Peer "p0") (T0 := Unit).
+    + apply U_Unit.
+    + apply U_Unit.
+    + apply T_Unit.
+    + apply T_Var. left. reflexivity.
     + reflexivity.
-    + { apply T_Comp with (P0 := Peer "p0") (T0 := Unit).
-        - apply U_Unit.
-        - apply U_Unit.
-        - reflexivity.
-        - apply T_Unit.
-        - apply T_Var. left. reflexivity.
-        - reflexivity.
-        - reflexivity.
-      }
+    + reflexivity.
 Qed.
 
 
 Example test_hasType_TCompFrom_single_1:
-    (* ensure test setup is correct ... *)
-    getPeer testPeerTyping1Ties1Context = Peer "p0" /\
-    getPeerType testPeerTyping1Ties1Context (PeerInst 2) = Some (Peer "ps") /\
-    getTieMult testPeerTyping1Ties1Context (Peer "p0", Peer "ps") = Some single /\
-    (* actual test ... *)
-    testPeerTyping1Ties1Context
-      |- asLocalInFrom (Id "x") (*=*) unit (*in*) unit (*:*) (Unit on (Peer "ps"))
-                       (*from*) (peerApp (PeerInst 2))
-      \in Unit.
+  (* ensure test setup is correct ... *)
+  testPeerTyping1 (PeerInst 2) = Some (Peer "ps") /\
+  testTies1 (Peer "p0", Peer "ps") = Some single /\
+  (* actual test ... *)
+  testPeerTyping1; testTies1; emptyReactEnv; emptyPlaceEnv; emptyVarEnv; Peer "p0"
+    |- asLocalInFrom (Id "x") (*=*) unit (*in*) unit (*:*) (Unit on (Peer "ps"))
+                     (*from*) (peerApp (PeerInst 2))
+    : Unit.
 Proof.
   split.
   - reflexivity.
   - split.
     + reflexivity.
-    + { split.
-        - reflexivity.
-        - apply T_ComFrom with (T0 := Unit) (P0 := Peer "p0").
-          + apply U_Unit.
-          + apply U_Unit.
-          + reflexivity.
-          + apply T_Unit.
-          + apply T_Unit.
-          + reflexivity.
-          + apply T_Peer. reflexivity.
-      }
+    + apply T_ComFrom with (T0 := Unit) (P0 := Peer "p0").
+      * apply U_Unit.
+      * apply U_Unit.
+      * apply T_Unit.
+      * apply T_Unit.
+      * reflexivity.
+      * apply T_Peer. reflexivity.
 Qed.
 
 
 Example test_hasType_TCompFrom_single_2:
-    (* ensure test setup is correct ... *)
-    getPeer testPeerTyping1Ties1Context = Peer "p0" /\
-    getPeerType testPeerTyping1Ties1Context (PeerInst 2) = Some (Peer "ps") /\
-    getTieMult testPeerTyping1Ties1Context (Peer "p0", Peer "ps") = Some single /\
-    (* actual test ... *)
-    testPeerTyping1Ties1Context
-      |- asLocalInFrom (Id "x") (*=*) unit (*in*) (idApp (Id "x"))
-                       (*:*) (Unit on (Peer "ps"))
-                       (*from*) (peerApp (PeerInst 2))
-      \in Unit.
+  (* ensure test setup is correct ... *)
+  testPeerTyping1 (PeerInst 2) = Some (Peer "ps") /\
+  testTies1 (Peer "p0", Peer "ps") = Some single /\
+  (* actual test ... *)
+  testPeerTyping1; testTies1; emptyReactEnv; emptyPlaceEnv; emptyVarEnv; Peer "p0"
+    |- asLocalInFrom (Id "x") (*=*) unit (*in*) (idApp (Id "x"))
+                     (*:*) (Unit on (Peer "ps"))
+                     (*from*) (peerApp (PeerInst 2))
+    : Unit.
 Proof.
   split.
   - reflexivity.
   - split.
     + reflexivity.
-    + { split.
-        - reflexivity.
-        - apply T_ComFrom with (T0 := Unit) (P0 := Peer "p0").
-          + apply U_Unit.
-          + apply U_Unit.
-          + reflexivity.
-          + apply T_Unit.
-          + apply T_Var. left. reflexivity.
-          + reflexivity.
-          + apply T_Peer. reflexivity.
-      }
+    + apply T_ComFrom with (T0 := Unit) (P0 := Peer "p0").
+      * apply U_Unit.
+      * apply U_Unit.
+      * apply T_Unit.
+      * apply T_Var. left. reflexivity.
+      * reflexivity.
+      * apply T_Peer. reflexivity.
 Qed.
 
 
 Example test_hasType_TReactive_1:
-    (* ensure test setup is correct ... *)
-    getReactType testReactContext1 (Reactive 0) = Some Unit /\
-    (* actual test ... *)
-    testReactContext1 |- (reactApp (Reactive 0)) \in Unit.
+  (* ensure test setup is correct ... *)
+  testPsi1 (Reactive 0) = Some Unit /\
+  (* actual test ... *)
+  noPeers; noTies; testPsi1; emptyPlaceEnv; emptyVarEnv; Peer "_" |- reactApp (Reactive 0) : Unit.
 Proof.
   split.
   - reflexivity.
@@ -446,15 +377,18 @@ Proof.
 Qed.
 
 
-Example test_hasType_TSignal_1: emptyContext |- signal unit \in Signal Unit.
+Example test_hasType_TSignal_1:
+  noPeers; noTies; emptyReactEnv; emptyPlaceEnv; emptyVarEnv; Peer "dummy" |- signal unit : Signal Unit.
 Proof. apply T_Signal. apply T_Unit. Qed.
 
 
-Example test_hasType_TReactiveVal_1: emptyContext |- var unit \in Var Unit.
+Example test_hasType_TReactiveVal_1:
+  noPeers; noTies; emptyReactEnv; emptyPlaceEnv; emptyVarEnv; Peer "dummy" |- var unit : Var Unit.
 Proof. apply T_ReactiveVar. apply T_Unit. Qed.
 
 
-Example test_hasType_TNow_signal_1: emptyContext |- now (signal unit) \in Unit.
+Example test_hasType_TNow_signal_1:
+  noPeers; noTies; emptyReactEnv; emptyPlaceEnv; emptyVarEnv; Peer "dummy" |- now (signal unit) : Unit.
 Proof.
   apply T_Now with (T0 := Signal Unit).
   - apply T_Signal. apply T_Unit.
@@ -462,7 +396,8 @@ Proof.
 Qed.
 
 
-Example test_hasType_TNow_var_1: emptyContext |- now (var unit) \in Unit.
+Example test_hasType_TNow_var_1:
+  noPeers; noTies; emptyReactEnv; emptyPlaceEnv; emptyVarEnv; Peer "dummy" |- now (var unit) : Unit.
 Proof.
   eapply T_Now.
   - apply T_ReactiveVar. apply T_Unit.
@@ -470,7 +405,8 @@ Proof.
 Qed.
 
 
-Example test_hasType_TSet_1: emptyContext |- set (var unit) unit \in Unit.
+Example test_hasType_TSet_1:
+  noPeers; noTies; emptyReactEnv; emptyPlaceEnv; emptyVarEnv; Peer "dummy" |- set (var unit) unit : Unit.
 Proof.
   apply T_Set with (T := Unit).
   - apply T_ReactiveVar. apply T_Unit.
@@ -479,14 +415,16 @@ Qed.
 
 
 Example test_hasType_TSet_2:
-  emptyContext |- set (var (lambda (Id "x") Unit unit))
-                      (*:=*) (lambda (Id "x") Unit unit)
-                \in Unit.
+  noPeers; noTies; emptyReactEnv; emptyPlaceEnv; emptyVarEnv; Peer "dummy"
+    |- set (var (lambda (Id "x") Unit unit))
+           (*:=*) (lambda (Id "x") Unit unit)
+    : Unit.
 Proof.
-  assert (H: emptyContext |- (lambda (Id "x") Unit unit) \in (Unit ~> Unit)).
-  { apply T_Abs. apply T_Unit. }
-  apply T_Set with (T := Unit ~> Unit).
-  - apply T_ReactiveVar. assumption.
-  - assumption.
+  assert (H: noPeers; noTies; emptyReactEnv; emptyPlaceEnv; emptyVarEnv; Peer "dummy" |- lambda (Id "x") Unit unit : Unit ~> Unit).
+  - apply T_Abs.
+    apply T_Unit.
+  - apply T_Set with (T := Unit ~> Unit).
+    + apply T_ReactiveVar. assumption.
+    + assumption.
 Qed.
 
